code/curve25519/Hacl.Spec.Bignum.Crecip.fst
@@ -22,22 +22,77 @@ let crecip_pre (z:seqelem) : GTot Type0 = red_513 z
 type s_513 = s:seqelem{red_513 s}
 
 
+#set-options "--initial_fuel 0 --max_fuel 0 --z3rlimit 10"
+
 inline_for_extraction private val fmul_tot: input:s_513 -> input2:s_513 -> Tot s_513
 inline_for_extraction private let fmul_tot input input2 =
   lemma_513_is_53 input; lemma_513_is_55 input2; fmul_53_55_is_fine input input2;
   fmul_tot input input2
   
+val lemma_fsquare_times_tot_def_0: s:seqelem{red_5413 s} -> Lemma
+  (fsquare_pre s /\ fsquare_times_tot s 1 == fsquare_spec s)
+#reset-options "--initial_fuel 1 --max_fuel 1"
+let lemma_fsquare_times_tot_def_0 s =
+  fsquare_5413_is_fine s
+
+#reset-options "--initial_fuel 0 --max_fuel 0"
+
+val lemma_fsquare_times_tot_def_1: s:seqelem{red_5413 s} -> n:nat{n > 1} -> Lemma
+  (fsquare_pre s /\ red_5413 (fsquare_spec s) /\
+    fsquare_times_tot s n == fsquare_times_tot (fsquare_spec s) (n-1))
+#reset-options "--initial_fuel 1 --max_fuel 1"
+let lemma_fsquare_times_tot_def_1 s n =
+  fsquare_5413_is_fine s;
+  lemma_513_is_5413 (fsquare_spec s)
+
+#reset-options "--initial_fuel 0 --max_fuel 0"
+
+val lemma_fsquare_times_tot: s:seqelem{red_5413 s} -> n:pos -> Lemma
+  (requires (True))
+  (ensures (selem (fsquare_times_tot s n) == Hacl.Spec.Bignum.Crecip.Lemmas.exp (selem s) (pow2 n)))
+  (decreases n)
+#reset-options "--initial_fuel 0 --max_fuel 0 --z3rlimit 100"
+let rec lemma_fsquare_times_tot s n =
+  fsquare_5413_is_fine s;
+  if n = 1 then (
+    assert_norm (pow2 1 = 2);
+    lemma_fsquare_times_tot_def_0 s;
+    Hacl.Spec.Bignum.Crecip.Lemmas.lemma_exp_def_1 (selem s) 2;
+    Hacl.Spec.Bignum.Crecip.Lemmas.lemma_exp_def_1 (selem s) 1;
+    Hacl.Spec.Bignum.Crecip.Lemmas.lemma_exp_def_0 (selem s);
+    Math.Lemmas.modulo_lemma (selem s) prime
+  ) else (
+    let s' = fsquare_spec s in
+    lemma_fsquare_times_tot_def_1 s n;
+    lemma_fsquare_times_tot s' (n-1);
+    cut (selem (fsquare_times_tot s' (n-1)) == Hacl.Spec.Bignum.Crecip.Lemmas.exp (selem s *@ selem s) (pow2 (n-1)));
+    Hacl.Spec.Bignum.Crecip.Lemmas.lemma_exp_double (selem s) (pow2 (n-1));
+    Math.Lemmas.pow2_double_sum (n-1)
+  )
+
+
+unfold inline_for_extraction
+val fsquare_times_tot: s:seqelem{red_513 s} -> n:pos -> Tot (s':seqelem{red_513 s' /\
+  selem s' == Hacl.Spec.Bignum.Crecip.Lemmas.exp (selem s) (pow2 n)})
+unfold inline_for_extraction
+let fsquare_times_tot s n =
+  lemma_513_is_5413 s;
+  lemma_fsquare_times_tot s n;
+  fsquare_times_tot s n
+
+module L = Hacl.Spec.Bignum.Crecip.Lemmas
 
 val crecip_tot_1: z:seqelem{red_513 z} -> Tot (s_513 * s_513 * s_513)
 let crecip_tot_1 z =
-  let a = fsquare_times_tot z 1 in
-  let t0 = fsquare_times_tot a 2 in
-  let b = fmul_tot t0 z in
-  let a' = fmul_tot b a in
-  let t0' = fsquare_times_tot a' 1 in
-  let b' = fmul_tot t0' b in
-  let t0'' = fsquare_times_tot b' 5 in
+  let a = fsquare_times_tot z 1 in  // z^2
+  let t0 = fsquare_times_tot a 2 in // z^8
+  let b = fmul_tot t0 z in          // z^9
+  let a' = fmul_tot b a in          // z^11
+  let t0' = fsquare_times_tot a' 1 in // z^22
+  let b' = fmul_tot t0' b in          // z^(2^5 - 2^0)
+  let t0'' = fsquare_times_tot b' 5 in // z^(2^10 - 2^5)
   t0'', b', a'
+
 
 
 #set-options "--initial_fuel 0 --max_fuel 0 --z3rlimit 20"
